some refactoring of auto elim pure

pulse/lib/steel/pulse/Pulse.Checker.Auto.ElimPure.fst
@@ -57,62 +57,105 @@ let elim_pure_typing (g:env) (p:host_term)
      T_STApp g elim_pure_head (tm_fstar (`(prop))) None (elim_pure_comp p) _ (elim_pure_head_typing g) p_prop
 
 #push-options "--query_stats --fuel 2 --ifuel 2 --split_queries no --z3rlimit_factor 4"
+let continuation_elaborator_with_bind (#g:env) (ctxt:term)
+  (#c1:comp{stateful_comp c1})
+  (#e1:st_term)
+  (e1_typing:st_typing g e1 c1)
+  (ctxt_pre1_typing:tot_typing g (Tm_Star ctxt (comp_pre c1)) Tm_VProp)
+  : T.Tac (x:var { None? (lookup g x) } &
+           continuation_elaborator
+             g (Tm_Star ctxt (comp_pre c1))
+             (extend x (Inl (comp_res c1)) g) (Tm_Star (open_term (comp_post c1) x) ctxt)) =
+
+  let pre1 = comp_pre c1 in
+  let res1 = comp_res c1 in
+  let post1 = comp_post c1 in
+  let ctxt_typing, pre1_typing = star_typing_inversion ctxt_pre1_typing in
+  // let p_prop = Metatheory.pure_typing_inversion pure_typing in
+  let v_eq = VE_Comm g ctxt pre1 in
+  let framing_token : F.frame_for_req_in_ctxt g (Tm_Star ctxt pre1) pre1 = 
+    (| ctxt, ctxt_typing, VE_Comm g pre1 ctxt  |)
+  in
+  let (| c1, e1_typing |) =
+    Pulse.Checker.Framing.apply_frame ctxt_pre1_typing e1_typing framing_token in
+  let (| u_of_1, pre_typing, _, _ |) =
+    Metatheory.(st_comp_typing_inversion (comp_typing_inversion (st_typing_correctness e1_typing))) in
+  let x = fresh g in
+  let b = Inl res1 in
+  let g' = extend x b g in
+  
+  let post1_opened = open_term_nv post1 (v_as_nv x) in
+  let k : continuation_elaborator g (Tm_Star ctxt pre1) g' (Tm_Star post1_opened ctxt) =
+    fun post_hint res ->
+    let (| e2, c2, e2_typing |) = res in
+    if not (stateful_comp c2) // || None? post_hint
+    then T.fail "Unexpected non-stateful comp in continuation elaborate"
+    else (
+      let e2_typing : st_typing g' e2 c2 = e2_typing in
+      let e2_closed = close_st_term e2 x in
+      assume (open_st_term e2_closed x == e2);
+      assert (comp_pre c1 == (Tm_Star ctxt pre1));
+      assert (comp_post c1 == Tm_Star post1 ctxt);
+      assert (comp_pre c2 == Tm_Star post1_opened ctxt);
+      assert (open_term (comp_post c1) x == Tm_Star post1_opened (open_term ctxt x));
+      // ctxt is well-typed, hence ln
+      assume (open_term ctxt x == ctxt);
+      assert (open_term (comp_post c1) x == comp_pre c2);
+      // e2 is well-typed in g, so its fvs should be a subset of g
+      assume (~ (x `Set.mem` freevars_st e2));
+      if x `Set.mem` freevars (comp_post c2)
+      then T.fail "Impossible"
+      else (
+        let t_typing, post_typing =
+          Pulse.Checker.Bind.bind_res_and_post_typing g (st_comp_of_comp c2) x post_hint in
+        let (| e, c, e_typing |) =
+          Pulse.Checker.Bind.mk_bind
+            g (Tm_Star ctxt pre1) 
+            e1 e2_closed c1 c2 (v_as_nv x) e1_typing
+            u_of_1 
+            e2_typing
+            t_typing
+            post_typing
+        in
+        (| e, c, e_typing |)
+      )
+    )
+
+  in
+  (| x, k |)
+
 let elim_one_pure (#g:env) (ctxt:term) (p:term)
                   (ctxt_p_typing:tot_typing g (Tm_Star ctxt (Tm_Pure p)) Tm_VProp)
-   : T.Tac (g':env { env_extends g' g } &
-            tot_typing g' ctxt Tm_VProp &
-            continuation_elaborator g (Tm_Star ctxt (Tm_Pure p)) g' ctxt)
-   = let ctxt_typing, pure_typing = star_typing_inversion ctxt_p_typing in
-     let p_prop = Metatheory.pure_typing_inversion pure_typing in
-     let v_eq = VE_Comm g ctxt (Tm_Pure p) in
-     let framing_token : F.frame_for_req_in_ctxt g (Tm_Star ctxt (Tm_Pure p)) (Tm_Pure p) = 
-        (| ctxt, ctxt_typing, VE_Comm g (Tm_Pure p) ctxt  |)
-     in
-     match p with
-     | Tm_FStar pp _ ->
-       let e1 =  (mk_elim_pure (tm_fstar pp)) in
-       let (| c1, e1_typing |) = Pulse.Checker.Framing.apply_frame ctxt_p_typing (elim_pure_typing g pp p_prop) framing_token in
-       let (| u_of_1, pre_typing, _, _ |) = Metatheory.(st_comp_typing_inversion (comp_typing_inversion (st_typing_correctness e1_typing))) in
-       let x = fresh g in
-       let b = Inl (comp_res c1) in
-       let g' = extend x b g in
-       let k : continuation_elaborator g (Tm_Star ctxt (Tm_Pure p)) g' (Tm_Star Tm_Emp ctxt) =
-           fun post_hint res -> 
-               let (| e2, c2, e2_typing |) = res in
-                if not (stateful_comp c2) // || None? post_hint
-                then T.fail "Unexpected non-stateful comp in continuation elaborate"
-                else (
-                    let e2_typing : st_typing g' e2 c2 = e2_typing in
-                    let e2_closed = close_st_term e2 x in
-                    assume (open_st_term e2_closed x == e2);
-                    assert (comp_pre c1 == (Tm_Star ctxt (Tm_Pure p)));
-                    assert (comp_post c1 == Tm_Star Tm_Emp ctxt);
-                    assert (comp_pre c2 == Tm_Star Tm_Emp ctxt); 
-                    assume (open_term (comp_post c1) x == comp_post c1);
-                    if x `Set.mem` freevars (comp_post c2)
+  : T.Tac (g':env { env_extends g' g } &
+           tot_typing g' ctxt Tm_VProp &
+           continuation_elaborator g (Tm_Star ctxt (Tm_Pure p)) g' ctxt) =
+  
+  let ctxt_typing, pure_typing = star_typing_inversion ctxt_p_typing in
+  let p_prop = Metatheory.pure_typing_inversion pure_typing in
 
-                    then T.fail "Impossible"
-                    else (
-                        let t_typing, post_typing =
-                          Pulse.Checker.Bind.bind_res_and_post_typing g (st_comp_of_comp c2) x post_hint in
-                        let (| e, c, e_typing |) =
-                            Pulse.Checker.Bind.mk_bind
-                                g (Tm_Star ctxt (Tm_Pure p)) 
-                                e1 e2_closed _ _ (v_as_nv x) e1_typing
-                                u_of_1 
-                                e2_typing
-                                t_typing
-                                post_typing
-                        in
-                        (| e, c, e_typing |)
-                    )
-                )
+  match p with
+  | Tm_FStar pp _ ->
+    let e1 = mk_elim_pure (tm_fstar pp) in
+    let c1 = elim_pure_comp pp in
+    let e1_typing = elim_pure_typing g pp p_prop in
+    let (| x, k |) = continuation_elaborator_with_bind ctxt e1_typing ctxt_p_typing in
+    let g' = extend x (Inl (comp_res c1)) g in
+    let ctxt_g'_typing : tot_typing g' ctxt Tm_VProp =
+      Metatheory.tot_typing_weakening x (Inl (comp_res c1)) ctxt_typing in
+    let k
+      : continuation_elaborator
+          g (Tm_Star ctxt (Tm_Pure p))
+          g' (Tm_Star Tm_Emp ctxt) =
+      k in
+    let k
+      : continuation_elaborator
+          g (Tm_Star ctxt (Tm_Pure p))
+          g' ctxt =
+      k_elab_equiv k (VE_Refl _ _) (VE_Unit _ ctxt) in
+    Pulse.Checker.Common.extends_extends_env g x (Inl (comp_res c1));
+    (| g', ctxt_g'_typing, k |)
 
-       in
-       let k = k_elab_equiv k (VE_Refl _ _) (VE_Unit _ ctxt) in
-       Pulse.Checker.Common.extends_extends_env g x b;
-       (| g', Metatheory.tot_typing_weakening x b ctxt_typing, k |)
-     | _ -> T.fail "unexpected pure term"
+  | _ -> T.fail "unexpected pure term"
 
 let rec elim_pure_right (#g:env) (#ctxt:term) (ctxt_typing:tot_typing g ctxt Tm_VProp)
    : T.Tac (g':env { env_extends g' g } &
@@ -130,51 +173,59 @@ let rec elim_pure_right (#g:env) (#ctxt:term) (ctxt_typing:tot_typing g ctxt Tm_
 
 module F = Pulse.Checker.Framing
 open Pulse.Checker.VPropEquiv
-                        
-let rec canon_pure_right_aux (g:env) (vps:list vprop)
-  : vps':list vprop &
-    pures:list vprop &
-    vprop_equiv g (list_as_vprop vps) (list_as_vprop (vps' @ pures))
-  = match vps with
-    | [] -> (| [], [], VE_Refl _ _ |)
-    | [Tm_Pure p] -> (| [], [Tm_Pure p], VE_Refl _ _ |)
-    | Tm_Pure p :: rest -> 
-      let (| vps', pures, v_eq |) = canon_pure_right_aux g rest in
+
+let rec canon_right_aux (g:env) (vps:list vprop) (f:vprop -> bool)
+  : vps' : list vprop &
+    fvps : list vprop { forall (v:vprop). List.Tot.memP v fvps ==> f v } &
+    vprop_equiv g (list_as_vprop vps) (list_as_vprop (vps' @ fvps)) =
+
+  match vps with
+  | [] -> (| [], [], VE_Refl _ _ |)
+  | hd::rest ->
+    if f hd
+    then begin
+      let (| vps', fvps, v_eq |) = canon_right_aux g rest f in
       let v_eq
-         : vprop_equiv g (list_as_vprop vps)
-                         (list_as_vprop ((Tm_Pure p) :: (vps' @ pures)))
-         = list_as_vprop_ctx g [Tm_Pure p] _ rest (vps' @ pures) (VE_Refl _ _) v_eq    
+        : vprop_equiv g (list_as_vprop vps)
+                        (list_as_vprop (hd :: (vps' @ fvps)))
+        = list_as_vprop_ctx g [hd] _ rest (vps' @ fvps) (VE_Refl _ _) v_eq    
       in  
       let v_eq
-         : vprop_equiv g (list_as_vprop vps)
-                         (list_as_vprop ((vps'@[Tm_Pure p]) @ pures))
-         = VE_Trans _ _ _ _ v_eq (VE_Sym _ _ _ (vprop_equiv_swap_equiv _ _ _ (Tm_Pure p) _ (VE_Refl _ _)))
+        : vprop_equiv g (list_as_vprop vps)
+                        (list_as_vprop ((vps'@[hd]) @ fvps))
+        = VE_Trans _ _ _ _ v_eq (VE_Sym _ _ _ (vprop_equiv_swap_equiv _ _ _ hd _ (VE_Refl _ _)))
       in
       let v_eq 
         :  vprop_equiv g (list_as_vprop vps)
-                         (list_as_vprop (vps'@(Tm_Pure p::pures)))
+                         (list_as_vprop (vps'@(hd::fvps)))
         = VE_Trans _ _ _ _ v_eq (VE_Sym _ _ _ (list_as_vprop_assoc _ _ _ _)) in
-      (| vps', Tm_Pure p :: pures, v_eq |)
-    | hd::rest ->
-      let (| vps', pures, v_eq |) = canon_pure_right_aux g rest in
+      (| vps', hd :: fvps, v_eq |)
+    end
+    else begin
+      let (| vps', pures, v_eq |) = canon_right_aux g rest f in
       let v_eq = list_as_vprop_ctx g [hd] _ _ _ (VE_Refl _ _) v_eq in
       (| hd::vps', pures, v_eq |)
+    end
 
+let canon_right (#g:env) (#ctxt:term) (ctxt_typing:tot_typing g ctxt Tm_VProp)
+  (f:vprop -> bool)
+  : (ctxt':term &
+     tot_typing g ctxt' Tm_VProp &
+     continuation_elaborator g ctxt g ctxt')
+  = let ctxt' = canon_vprop ctxt in
+    let (| vps', pures, veq |) = canon_right_aux g (vprop_as_list ctxt) f in
+    let veq : vprop_equiv g ctxt (list_as_vprop (vps'@pures)) =
+        VE_Trans _ _ _ _ (vprop_list_equiv g ctxt) veq
+    in
+    (| _, VP.vprop_equiv_typing_fwd ctxt_typing veq, k_elab_equiv (k_elab_unit _ _) (VE_Refl _ _) veq |)
 
 
 let canon_pure_right (#g:env) (#ctxt:term) (ctxt_typing:tot_typing g ctxt Tm_VProp)
   : (ctxt':term &
      tot_typing g ctxt' Tm_VProp &
      continuation_elaborator g ctxt g ctxt')
-  = let ctxt' = canon_vprop ctxt in
-    let (| vps', pures, veq |) = canon_pure_right_aux g (vprop_as_list ctxt) in
-    let veq : vprop_equiv g ctxt (list_as_vprop (vps'@pures)) =
-        VE_Trans _ _ _ _ (vprop_list_equiv g ctxt) veq
-    in
-    (| _, VP.vprop_equiv_typing_fwd ctxt_typing veq, k_elab_equiv (k_elab_unit _ _) (VE_Refl _ _) veq |)
+  = canon_right ctxt_typing Tm_Pure?
 
-  
-                
 let elim_pure (#g:env) (#ctxt:term) (ctxt_typing:tot_typing g ctxt Tm_VProp)
    : T.Tac (g':env { env_extends g' g } &
             ctxt':term &
