pulse/lib/steel/pulse/Pulse.Checker.Auto.Util.fsti
@@ -11,7 +11,7 @@ val k_elab_trans (#g0 #g1 #g2:env) (#ctxt0 #ctxt1 #ctxt2:term)
                  (k1:continuation_elaborator g1 ctxt1 g2 ctxt2 { g1 `env_extends` g0})
    : continuation_elaborator g0 ctxt0 g2 ctxt2
 
-val k_elab_equiv (#g1 #g2:env) (#ctxt1 #ctxt1' #ctxt2 #ctxt2':term)                 
+val k_elab_equiv (#g1 #g2:env) (#ctxt1 #ctxt1' #ctxt2 #ctxt2':term)
                  (k:continuation_elaborator g1 ctxt1 g2 ctxt2)
                  (d1:vprop_equiv g1 ctxt1 ctxt1')
                  (d2:vprop_equiv g2 ctxt2 ctxt2')
